
$P \leftrightarrow Q \equiv \neg P \leftrightarrow \neg Q$

\begin{align*}
  &P \leftrightarrow Q &(Begin)\\
  &\equiv (P \rightarrow Q) \land (Q \rightarrow P) &(\textrm{definition of
    bi-directionality})\\
  &\equiv (\neg P \lor Q) \land (\neg Q \lor P) &(\textrm{Conditional Law})\\
  &\equiv (Q \lor \neg P) \land (P \lor \neg Q) &(\textrm{Commutative Law})\\
  &\equiv (\neg Q \rightarrow \neg P) \land (\neg P \rightarrow \neg Q)
    &(\textrm{Conditional Law})\\
  &\equiv \neg P \leftrightarrow \neg Q &(\textrm{definition of bi-directionality})\\
\end{align*}
